theories/channel/channel.v
@@ -67,8 +67,8 @@ Section channel.
 
   Definition chan_inv (γ : chan_name) (l r : loc) : iProp Σ :=
     (∃ ls rs,
-      llist l ls ∗ own (chan_l_name γ) (● to_auth_excl ls) ∗
-      llist r rs ∗ own (chan_r_name γ) (● to_auth_excl rs))%I.
+      llist sbi_internal_eq l ls ∗ own (chan_l_name γ) (● to_auth_excl ls) ∗
+      llist sbi_internal_eq r rs ∗ own (chan_r_name γ) (● to_auth_excl rs))%I.
   Typeclasses Opaque chan_inv.
 
   Definition is_chan (γ : chan_name) (c1 c2 : val) : iProp Σ :=
@@ -99,8 +99,8 @@ Section channel.
     iMod (own_alloc (● (to_auth_excl []) ⋅ ◯ (to_auth_excl []))) as (rsγ) "[Hrs Hrs']".
     { by apply auth_both_valid. }
     wp_apply (newlock_spec N (∃ ls rs,
-      llist l ls ∗ own lsγ (● to_auth_excl ls) ∗
-      llist r rs ∗ own rsγ (● to_auth_excl rs))%I with "[Hl Hr Hls Hrs]").
+      llist sbi_internal_eq l ls ∗ own lsγ (● to_auth_excl ls) ∗
+      llist sbi_internal_eq r rs ∗ own rsγ (● to_auth_excl rs))%I with "[Hl Hr Hls Hrs]").
     { eauto 10 with iFrame. }
     iIntros (lk γlk) "#Hlk". wp_pures.
     iApply ("HΦ" $! _ _ (Chan_name γlk lsγ rsγ)); simpl.
@@ -109,9 +109,9 @@ Section channel.
 
   Lemma chan_inv_alt s γ l r :
     chan_inv γ l r ⊣⊢ ∃ ls rs,
-      llist (side_elim s l r) ls ∗
+      llist sbi_internal_eq (side_elim s l r) ls ∗
       own (side_elim s chan_l_name chan_r_name γ) (● to_auth_excl ls) ∗
-      llist (side_elim s r l) rs ∗
+      llist sbi_internal_eq (side_elim s r l) rs ∗
       own (side_elim s chan_r_name chan_l_name γ) (● to_auth_excl rs).
   Proof.
     destruct s; rewrite /chan_inv //=.
@@ -137,7 +137,7 @@ Section channel.
     iDestruct (excl_eq with "Hvs Hchan") as %<-%leibniz_equiv.
     iMod (excl_update _ _ _ (vs ++ [v]) with "Hvs Hchan") as "[Hvs Hchan]".
     wp_pures. iMod ("HΦ" with "Hchan") as "HΦ"; iModIntro.
-    wp_apply (lsnoc_spec with "Hll"); iIntros "Hll".
+    wp_apply (lsnoc_spec with "[$Hll //]"); iIntros "Hll".
     wp_apply (release_spec with "[-HΦ $Hlock $Hlocked]"); last eauto.
     iApply (chan_inv_alt s).
     rewrite /llist. eauto 20 with iFrame.
@@ -171,7 +171,7 @@ Section channel.
       iMod (excl_update _ _ _ vs with "Hvs Hvs'") as "[Hvs Hvs']".
       wp_pures. iMod ("HΦ" with "[//] Hvs'") as "HΦ"; iModIntro.
       wp_apply (lisnil_spec with "Hll"); iIntros "Hll".
-      wp_apply (lpop_spec with "Hll"); iIntros "Hll".
+      wp_apply (lpop_spec with "Hll"); iIntros (v') "[% Hll]"; simplify_eq/=.
       wp_apply (release_spec with "[-HΦ $Hlocked $Hlock]").
       { iApply (chan_inv_alt s).
         rewrite /llist. eauto 10 with iFrame. }
