theories/examples/sort.v
@@ -34,47 +34,42 @@ Section sort.
     (<!> A (I : A → val → iProp Σ) (R : A → A → Prop)
          `{!RelDecision R, !Total R} (cmp : val),
        MSG cmp {{ cmp_spec I R cmp }};
-     <!> (xs : list A) (l : loc) (vs : list val),
-       MSG #l {{ llist l vs ∗ [∗ list] x;v ∈ xs;vs, I x v }};
-     <?> (xs' : list A) (vs' : list val),
-       MSG #() {{ ⌜ Sorted R xs' ⌝ ∗ ⌜ xs' ≡ₚ xs ⌝ ∗
-                  llist l vs' ∗ [∗ list] x;v ∈ xs';vs', I x v }};
+     <!> (xs : list A) (l : loc), MSG #l {{ llist I l xs }};
+     <?> (xs' : list A), MSG #() {{ ⌜ Sorted R xs' ⌝ ∗ ⌜ xs' ≡ₚ xs ⌝ ∗ llist I l xs' }};
      END)%proto.
 
   Lemma lmerge_spec {A} (I : A → val → iProp Σ) (R : A → A → Prop)
-      `{!RelDecision R, !Total R} (cmp : val) l1 l2 xs1 xs2 vs1 vs2 :
+      `{!RelDecision R, !Total R} (cmp : val) l1 l2 xs1 xs2 :
     cmp_spec I R cmp -∗
-    {{{
-      llist l1 vs1 ∗ llist l2 vs2 ∗
-      ([∗ list] x;v ∈ xs1;vs1, I x v) ∗ ([∗ list] x;v ∈ xs2;vs2, I x v)
-    }}}
+    {{{ llist I l1 xs1 ∗ llist I l2 xs2 }}}
       lmerge cmp #l1 #l2
-    {{{ ws, RET #(); llist l1 ws ∗ [∗ list] x;v ∈ list_merge R xs1 xs2;ws, I x v }}}.
+    {{{ RET #(); llist I l1 (list_merge R xs1 xs2) }}}.
   Proof.
-    iIntros "#Hcmp" (Ψ) "!> (Hl1 & Hl2 & HI1 & HI2) HΨ".
-    iLöb as "IH" forall (l2 xs1 xs2 vs1 vs2 Ψ).
+    iIntros "#Hcmp" (Ψ) "!> [Hl1 Hl2] HΨ".
+    iLöb as "IH" forall (l2 xs1 xs2 Ψ).
     wp_lam. wp_apply (lisnil_spec with "Hl1"); iIntros "Hl1".
-    destruct xs1 as [|x1 xs1], vs1 as [|v1 vs1]; simpl; done || wp_pures.
+    destruct xs1 as [|x1 xs1]; wp_pures.
     { wp_apply (lapp_spec with "[$Hl1 $Hl2]"); iIntros "[Hl1 _] /=".
       iApply "HΨ". iFrame. by rewrite list_merge_nil_l. }
     wp_apply (lisnil_spec with "Hl2"); iIntros "Hl2".
-    destruct xs2 as [|x2 xs2], vs2 as [|v2 vs2]; simpl; done || wp_pures.
+    destruct xs2 as [|x2 xs2]; wp_pures.
     { iApply "HΨ". iFrame. }
-    wp_apply (lhead_spec with "Hl1"); iIntros "Hl1".
-    wp_apply (lhead_spec with "Hl2"); iIntros "Hl2".
-    iDestruct "HI1" as "[HI1 HI1']"; iDestruct "HI2" as "[HI2 HI2']".
-    wp_apply ("Hcmp" with "[$HI1 $HI2]"); iIntros "[HI1 HI2]".
+    wp_apply (lhead_spec_aux with "Hl1"); iIntros (v1 l1') "[HIx1 Hl1]".
+    wp_apply (lhead_spec_aux with "Hl2"); iIntros (v2 l2') "[HIx2 Hl2]".
+    wp_apply ("Hcmp" with "[$HIx1 $HIx2]"); iIntros "[HIx1 HIx2] /=".
     case_bool_decide; wp_pures.
     - rewrite decide_True //.
-      wp_apply (lpop_spec with "Hl1"); iIntros "Hl1".
-      wp_apply ("IH" $! _ _ (x2 :: _) with "Hl1 Hl2 HI1' [$HI2 $HI2']").
-      iIntros (ws) "[Hl1 HI]".
-      wp_apply (lcons_spec with "Hl1"); iIntros "Hl1". iApply "HΨ". iFrame.
+      wp_apply (lpop_spec_aux with "Hl1"); iIntros "Hl1".
+      wp_apply ("IH" $! _ _ (_ :: _) with "Hl1 [HIx2 Hl2]").
+      { iExists _, _. iFrame. }
+      iIntros "Hl1".
+      wp_apply (lcons_spec with "[$Hl1 $HIx1]"). iIntros "Hl1". iApply "HΨ". iFrame.
     - rewrite decide_False //.
-      wp_apply (lpop_spec with "Hl2"); iIntros "Hl2".
-      wp_apply ("IH" $! _ (x1 :: _) with "Hl1 Hl2 [$HI1 $HI1'] HI2'").
-      iIntros (ws) "[Hl1 HI]".
-      wp_apply (lcons_spec with "Hl1"); iIntros "Hl1". iApply "HΨ". iFrame.
+      wp_apply (lpop_spec_aux with "Hl2"); iIntros "Hl2".
+      wp_apply ("IH" $! _ (_ :: _) with "[HIx1 Hl1] Hl2").
+      { iExists _, _. iFrame. }
+      iIntros "Hl1".
+      wp_apply (lcons_spec with "[$Hl1 $HIx2]"); iIntros "Hl1". iApply "HΨ". iFrame.
   Qed.
 
   Lemma sort_service_spec p c :
@@ -84,16 +79,14 @@ Section sort.
   Proof.
     iIntros (Ψ) "Hc HΨ". iLöb as "IH" forall (p c Ψ). wp_lam.
     wp_recv (A I R ?? cmp) as "#Hcmp".
-    wp_recv (xs l vs) as "[Hl HI]".
+    wp_recv (xs l) as "Hl".
     wp_apply (llength_spec with "Hl"); iIntros "Hl".
-    iDestruct (big_sepL2_length with "HI") as %<-.
     wp_op; case_bool_decide as Hlen; wp_if.
     { assert (Sorted R xs).
       { destruct xs as [|x1 [|x2 xs]]; simpl in *; eauto with lia. }
-      wp_send with "[$Hl $HI]"; first by auto. by iApply "HΨ". }
+      wp_send with "[$Hl]"; first by auto. by iApply "HΨ". }
     wp_apply (lsplit_spec with "Hl"); iIntros (l2 vs1 vs2);
       iDestruct 1 as (->) "[Hl1 Hl2]".
-    iDestruct (big_sepL2_app_inv_r with "HI") as (xs1 xs2 ->) "[HI1 HI2]".
     wp_apply (start_chan_proto_spec N sort_protocol); iIntros (cy) "Hcy".
     { rewrite -{2}(right_id END%proto _ (iProto_dual _)).
       wp_apply ("IH" with "Hcy"); auto. }
@@ -101,13 +94,13 @@ Section sort.
     { rewrite -{2}(right_id END%proto _ (iProto_dual _)).
       wp_apply ("IH" with "Hcz"); auto. }
     wp_send with "[$Hcmp]".
-    wp_send with "[$Hl1 $HI1]".
+    wp_send with "[$Hl1]".
     wp_send with "[$Hcmp]".
-    wp_send with "[$Hl2 $HI2]".
-    wp_recv (ys1 ws1) as (??) "[Hl1 HI1]".
-    wp_recv (ys2 ws2) as (??) "[Hl2 HI2]".
-    wp_apply (lmerge_spec with "Hcmp [$Hl1 $Hl2 $HI1 $HI2]"); iIntros (ws) "[Hl HI]".
-    wp_send ((list_merge R ys1 ys2) ws) with "[$Hl $HI]".
+    wp_send with "[$Hl2]".
+    wp_recv (ys1) as (??) "Hl1".
+    wp_recv (ys2) as (??) "Hl2".
+    wp_apply (lmerge_spec with "Hcmp [$Hl1 $Hl2]"); iIntros "Hl".
+    wp_send ((list_merge R ys1 ys2)) with "[$Hl]".
     - iSplit; iPureIntro.
       + by apply (Sorted_list_merge _).
       + rewrite (merge_Permutation R). by f_equiv.
