theories/examples/sort_client.v
@@ -12,12 +12,11 @@ Section sort_client.
   Context `{!heapG Σ, !proto_chanG Σ} (N : namespace).
 
   Lemma sort_client_spec {A} (I : A → val → iProp Σ) R
-       `{!RelDecision R, !Total R} cmp l (vs : list val) (xs : list A) :
+       `{!RelDecision R, !Total R} cmp l (xs : list A) :
     cmp_spec I R cmp -∗
-    {{{ llist l vs ∗ [∗ list] x;v ∈ xs;vs, I x v }}}
+    {{{ llist I l xs }}}
       sort_client cmp #l
-    {{{ ys ws, RET #(); ⌜Sorted R ys⌝ ∗ ⌜ys ≡ₚ xs⌝ ∗
-               llist l ws ∗ [∗ list] y;w ∈ ys;ws, I y w }}}.
+    {{{ ys, RET #(); ⌜Sorted R ys⌝ ∗ ⌜ys ≡ₚ xs⌝ ∗ llist I l ys }}}.
   Proof.
     iIntros "#Hcmp !>" (Φ) "Hl HΦ". wp_lam.
     wp_apply (start_chan_proto_spec N sort_protocol); iIntros (c) "Hc".
@@ -25,25 +24,7 @@ Section sort_client.
       wp_apply (sort_service_spec with "Hc"); auto. }
     wp_send with "[$Hcmp]".
     wp_send with "[$Hl]".
-    wp_recv (ys ws) as "(Hsorted & Hperm & Hl & HI)".
+    wp_recv (ys) as "(Hsorted & Hperm & Hl)".
     wp_pures. iApply "HΦ"; iFrame.
-  Qed.
-
-  Lemma sort_client_Zle_spec l (xs : list Z) :
-    {{{ llist l (LitV ∘ LitInt <$> xs) }}}
-      sort_client cmpZ #l
-    {{{ ys, RET #(); ⌜Sorted (≤) ys⌝ ∗ ⌜ ys ≡ₚ xs⌝ ∗ llist l (LitV ∘ LitInt <$> ys) }}}.
-  Proof.
-    iIntros (Φ) "Hl HΦ".
-    iApply (sort_client_spec IZ (≤) _ _ (LitV ∘ LitInt <$> xs) xs with "[] [Hl] [HΦ]").
-    { iApply cmpZ_spec. }
-    { iFrame "Hl". iInduction xs as [|x xs] "IH"; csimpl; by iFrame "#". }
-    iIntros "!>" (ys ws) "(?&?&?&HI)".
-    iAssert ⌜ ws = (LitV ∘ LitInt) <$> ys ⌝%I with "[HI]" as %->.
-    { iInduction ys as [|y ys] "IH" forall (ws);
-        destruct ws as [|w ws]; csimpl; try done.
-      iDestruct "HI" as "[-> HI2]".
-      by iDestruct ("IH" with "HI2") as %->. }
-    iApply ("HΦ" $! ys with "[$]").
   Qed.
 End sort_client.
