theories/examples/sort_elem_client.v
@@ -28,61 +28,56 @@ Section sort_elem_client.
   Context `{!heapG Σ, !proto_chanG Σ} (N : namespace).
   Context {A} (I : A → val → iProp Σ) (R : relation A) `{!RelDecision R, !Total R}.
 
-  Lemma send_all_spec c p xs' l xs vs :
-    {{{ llist l vs ∗ c ↣ sort_elem_head_protocol I R xs' <++> p @ N ∗ [∗ list] x;v ∈ xs;vs, I x v }}}
+  Lemma send_all_spec c p xs' l xs :
+    {{{ llist I l xs ∗ c ↣ sort_elem_head_protocol I R xs' <++> p @ N }}}
       send_all c #l
     {{{ RET #(); c ↣ sort_elem_head_protocol I R (xs' ++ xs) <++> p @ N }}}.
   Proof.
-    iIntros (Φ) "(Hl & Hc & HI) HΦ".
-    iInduction xs as [|x xs] "IH" forall (xs' vs); destruct vs as [|v vs]=>//.
+    iIntros (Φ) "[Hl Hc] HΦ".
+    iInduction xs as [|x xs] "IH" forall (xs').
     { wp_lam. wp_apply (lisnil_spec with "Hl"); iIntros "Hl"; wp_pures.
       iApply "HΦ". rewrite right_id_L. iFrame. }
-    iDestruct "HI" as "[HIxv HI]". wp_lam.
-    wp_apply (lisnil_spec with "Hl"); iIntros "Hl". wp_select.
-    wp_apply (lpop_spec with "Hl"); iIntros "Hl".
-    wp_send with "[$HIxv]". wp_apply ("IH" with "Hl Hc HI"). by rewrite -assoc_L.
+    wp_lam. wp_apply (lisnil_spec with "Hl"); iIntros "Hl". wp_select.
+    wp_apply (lpop_spec with "Hl"); iIntros (v) "[HIx Hl]".
+    wp_send with "[$HIx]". wp_apply ("IH" with "Hl Hc"). by rewrite -assoc_L.
   Qed.
 
   Lemma recv_all_spec c p xs ys' :
     Sorted R ys' →
     {{{ c ↣ sort_elem_tail_protocol I R xs ys' <++> p @ N }}}
       recv_all c
-    {{{ l ys ws, RET #l;
-        ⌜Sorted R (ys' ++ ys)⌝ ∗ ⌜ys' ++ ys ≡ₚ xs⌝ ∗
-        llist l ws ∗ c ↣ p @ N ∗ [∗ list] y;w ∈ ys;ws, I y w
+    {{{ l ys, RET #l;
+        ⌜Sorted R (ys' ++ ys)⌝ ∗ ⌜ys' ++ ys ≡ₚ xs⌝ ∗ llist I l ys ∗ c ↣ p @ N
     }}}.
   Proof.
     iIntros (Hsort Φ) "Hc HΦ".
     iLöb as "IH" forall (xs ys' Φ Hsort).
     wp_lam. wp_branch as %_ | %Hperm; wp_pures.
-    - wp_recv (y v) as (Htl) "HIxv".
+    - wp_recv (y v) as (Htl) "HIx".
       wp_apply ("IH" with "[] Hc"); first by auto using Sorted_snoc.
-      iIntros (l ys ws). rewrite -!assoc_L. iDestruct 1 as (??) "(Hl & Hc & HI)".
-      wp_apply (lcons_spec with "Hl"); iIntros "Hl"; wp_pures.
-      iApply ("HΦ" $! _ (y :: ys)); simpl; eauto with iFrame.
+      iIntros (l ys). rewrite -!assoc_L. iDestruct 1 as (??) "[Hl Hc]".
+      wp_apply (lcons_spec with "[$Hl $HIx]"); iIntros "Hl"; wp_pures.
+      iApply ("HΦ" with "[$Hl $Hc]"); simpl; eauto.
     - wp_apply (lnil_spec with "[//]"); iIntros (l) "Hl".
-      iApply ("HΦ" $! _ [] []); rewrite /= right_id_L; by iFrame.
+      iApply ("HΦ" $! _ []); rewrite /= right_id_L; by iFrame.
   Qed.
 
-  Lemma sort_client_spec cmp l vs xs :
+  Lemma sort_client_spec cmp l xs :
     cmp_spec I R cmp -∗
-    {{{ llist l vs ∗ [∗ list] x;v ∈ xs;vs, I x v }}}
+    {{{ llist I l xs }}}
       sort_elem_client cmp #l
-    {{{ k ys ws, RET #k;
-        ⌜Sorted R ys⌝ ∗ ⌜ys ≡ₚ xs⌝ ∗
-        llist k ws ∗ [∗ list] y;w ∈ ys;ws, I y w
-    }}}.
+    {{{ k ys, RET #k; ⌜Sorted R ys⌝ ∗ ⌜ys ≡ₚ xs⌝ ∗ llist I k ys }}}.
   Proof.
-    iIntros "#Hcmp !>" (Φ) "[Hl HI] HΦ". wp_lam.
+    iIntros "#Hcmp !>" (Φ) "Hl HΦ". wp_lam.
     wp_apply (start_chan_proto_spec N (sort_elem_top_protocol <++> END)%proto);
       iIntros (c) "Hc".
     { wp_apply (sort_elem_service_top_spec N with "Hc"); auto. }
     rewrite /sort_elem_top_protocol.
     wp_send (A I R) with "[$Hcmp]".
-    wp_apply (send_all_spec with "[$Hl $HI $Hc]"); iIntros "Hc".
+    wp_apply (send_all_spec with "[$Hl $Hc]"); iIntros "Hc".
     wp_select.
-    wp_apply (recv_all_spec _ _ _ [] with "[$Hc]"); auto.
-    iIntros (k ys ws) "/=". iDestruct 1 as (??) "(Hk & _ & HI)".
+    wp_apply (recv_all_spec with "Hc"); auto.
+    iIntros (k ys) "/=". iDestruct 1 as (??) "[Hk _]".
     iApply "HΦ"; auto with iFrame.
   Qed.
 End sort_elem_client.
